Sequential simulation compatibility

src/itree/SeqCompatibility.v
@@ -47,6 +47,8 @@ Require Import Simple.
 Require Import FlagAux.
 Require Import ITreeLang.
 
+Require Import SimAux.
+Require Import SeqAux.
 
 
 Definition SIM_VAL R_src R_tgt := forall (r_src:R_src) (r_tgt:R_tgt), Prop.
@@ -75,13 +77,11 @@ Definition _sim_itree
            R_src R_tgt
            (sim_ret:SIM_VAL R_src R_tgt)
            (itr_src: itree MemE.t R_src) (itr_tgt: itree MemE.t R_tgt): Prop :=
-  forall lc_src lc_tgt sc0_src sc0_tgt mem0_src mem0_tgt
-         (LOCAL: sim_local SimPromises.bot lc_src lc_tgt),
-    sim_seq_all
-      (lang R_src) (lang R_tgt)
-      (sim_terminal sim_ret)
-      itr_src lc_src sc0_src mem0_src
-      itr_tgt lc_tgt sc0_tgt mem0_tgt.
+  forall mem p,
+    @sim_seq (lang R_src) (lang R_tgt) (sim_terminal sim_ret)
+             p Flags.bot
+             (@SeqState.mk (lang R_src) itr_src mem)
+             (@SeqState.mk (lang R_tgt) itr_tgt mem).
 
 Definition _sim_ktree
            (sim_seq:SIM_SEQ)
@@ -95,14 +95,14 @@ Definition _sim_ktree
     _sim_itree sim_seq sim_ret1 (ktr_src r_src) (ktr_tgt r_tgt).
 
 Lemma _sim_itree_mon
-      s1 s2 (S: s1 <11= s2):
+      s1 s2 (S: s1 <7= s2):
   @_sim_itree s1 <5= @_sim_itree s2.
 Proof.
   ii. apply S. apply PR; auto.
 Qed.
 
 Lemma _sim_ktree_mon
-      s1 s2 (S: s1 <11= s2):
+      s1 s2 (S: s1 <7= s2):
   @_sim_ktree s1 <8= @_sim_ktree s2.
 Proof.
   ii. apply S. apply PR; auto.
@@ -119,63 +119,101 @@ Proof.
   rewrite bind_spin. econs; eauto.
 Qed.
 
-Lemma program_step_bind R0 R1
-      (itr0 itr1: itree MemE.t R0) (k: R0 -> itree MemE.t R1) e
-      lc1 sc1 mem1
-      lc2 sc2 mem2
-      (STEP: Thread.program_step
-               e
-               (Thread.mk (lang R0) itr0 lc1 sc1 mem1)
-               (Thread.mk (lang R0) itr1 lc2 sc2 mem2)):
-  Thread.program_step
-    e
-    (Thread.mk (lang R1) (itr0 >>= k) lc1 sc1 mem1)
-    (Thread.mk (lang R1) (itr1 >>= k) lc2 sc2 mem2).
+Lemma na_step_bind R0 R1
+      (itr0 itr1: itree MemE.t R0) (k: R0 -> itree MemE.t R1)
+      mem1 mem2 p e
+      (STEP: SeqState.na_step
+               p e
+               (@SeqState.mk (lang R0) itr0 mem1)
+               (@SeqState.mk (lang R0) itr1 mem2)):
+  SeqState.na_step
+    p e
+    (@SeqState.mk (lang R1) (itr0 >>= k) mem1)
+    (@SeqState.mk (lang R1) (itr1 >>= k) mem2).
 Proof.
-  inv STEP; inv LOCAL; ss.
-  - econs; [|econs 1]; s; eauto. apply lang_step_bind. auto.
-  - econs; [|econs 2]; s; eauto. apply lang_step_bind. auto.
-  - econs; [|econs 3]; s; eauto. apply lang_step_bind. auto.
-  - econs; [|econs 4]; s; eauto. apply lang_step_bind. auto.
-  - econs; [|econs 5]; s; eauto. apply lang_step_bind. auto.
-  - econs; [|econs 6]; s; eauto. apply lang_step_bind. auto.
-  - econs; [|econs 7]; s; eauto. apply lang_step_bind. auto.
-  - econs; [|econs 8]; s; eauto. apply lang_step_bind. auto.
-  - econs; [|econs 9]; s; eauto. apply lang_step_bind. auto.
-  - econs; [|econs 10]; s; eauto. apply lang_step_bind. auto.
-  - econs; [|econs 11]; s; eauto. apply lang_step_bind. auto.
+  inv STEP. econs; eauto.
+  apply lang_step_bind. auto.
 Qed.
 
-Lemma step_bind R0 R1
-      (itr0 itr1: itree MemE.t R0) (k: R0 -> itree MemE.t R1) pf e
-      lc1 sc1 mem1
-      lc2 sc2 mem2
-      (STEP: Thread.step pf e
-                         (Thread.mk (lang R0) itr0 lc1 sc1 mem1)
-                         (Thread.mk (lang R0) itr1 lc2 sc2 mem2)):
-  Thread.step pf e
-              (Thread.mk (lang R1) (itr0 >>= k) lc1 sc1 mem1)
-              (Thread.mk (lang R1) (itr1 >>= k) lc2 sc2 mem2).
+Lemma na_opt_step_bind R0 R1
+      (itr0 itr1: itree MemE.t R0) (k: R0 -> itree MemE.t R1)
+      mem1 mem2 p e
+      (STEP: SeqState.na_opt_step
+               p e
+               (@SeqState.mk (lang R0) itr0 mem1)
+               (@SeqState.mk (lang R0) itr1 mem2)):
+  SeqState.na_opt_step
+    p e
+    (@SeqState.mk (lang R1) (itr0 >>= k) mem1)
+    (@SeqState.mk (lang R1) (itr1 >>= k) mem2).
 Proof.
   inv STEP.
-  - econs 1. inv STEP0. econs; eauto.
-  - econs 2. apply program_step_bind. eauto.
+  { econs 1; eauto. eapply na_step_bind; eauto. }
+  { econs 2; eauto. }
 Qed.
 
-Lemma opt_step_bind R0 R1
-      (itr0 itr1: itree MemE.t R0) (k: R0 -> itree MemE.t R1) e
-      lc1 sc1 mem1
-      lc2 sc2 mem2
-      (STEP: Thread.opt_step e
-                             (Thread.mk (lang R0) itr0 lc1 sc1 mem1)
-                             (Thread.mk (lang R0) itr1 lc2 sc2 mem2)):
-  Thread.opt_step e
-                  (Thread.mk (lang R1) (itr0 >>= k) lc1 sc1 mem1)
-                  (Thread.mk (lang R1) (itr1 >>= k) lc2 sc2 mem2).
+Lemma rtc_na_step_bind R0 R1
+      (itr0 itr1: itree MemE.t R0) (k: R0 -> itree MemE.t R1)
+      mem1 mem2 p
+      (STEP: rtc (SeqState.na_step p MachineEvent.silent)
+                 (@SeqState.mk (lang R0) itr0 mem1)
+                 (@SeqState.mk (lang R0) itr1 mem2)):
+  rtc (SeqState.na_step p MachineEvent.silent)
+      (@SeqState.mk (lang R1) (itr0 >>= k) mem1)
+      (@SeqState.mk (lang R1) (itr1 >>= k) mem2).
 Proof.
-  inv STEP.
-  - econs 1.
-  - econs 2. apply step_bind. eauto.
+  remember (@SeqState.mk (lang R0) itr0 mem1).
+  remember (@SeqState.mk (lang R0) itr1 mem2).
+  revert itr0 itr1 mem1 mem2 Heqt Heqt0.
+  induction STEP; i; clarify.
+  { econs. }
+  { destruct y. econs.
+    { eapply na_step_bind; eauto. }
+    { eapply IHSTEP; eauto. }
+  }
+Qed.
+
+Lemma seq_thread_steps_bind R0 R1
+      (itr0 itr1: itree MemE.t R0) (k: R0 -> itree MemE.t R1)
+      mem0 mem1 p0 p1 o0 o1 tr
+      (STEPS: SeqThread.steps
+                (@SeqState.na_step _) tr
+                (SeqThread.mk (@SeqState.mk (lang R0) itr0 mem0) p0 o0)
+                (SeqThread.mk (@SeqState.mk (lang R0) itr1 mem1) p1 o1))
+  :
+    SeqThread.steps
+      (@SeqState.na_step _) tr
+      (@SeqThread.mk (lang R1) (@SeqState.mk (lang R1) (itr0 >>= k) mem0) p0 o0)
+      (@SeqThread.mk (lang R1) (@SeqState.mk (lang R1) (itr1 >>= k) mem1) p1 o1).
+Proof.
+  remember (SeqThread.mk (@SeqState.mk (lang R0) itr0 mem0) p0 o0).
+  remember (SeqThread.mk (@SeqState.mk (lang R0) itr1 mem1) p1 o1).
+  revert itr0 itr1 mem0 mem1 p0 p1 o0 o1 Heqt Heqt0.
+  induction STEPS; i; clarify; ss.
+  { econs 1. }
+  { inv STEP. destruct st1. econs 2.
+    { econs. eapply na_step_bind; eauto. }
+    { eapply IHSTEPS; eauto. }
+  }
+  { inv STEP. econs 3.
+    { econs; eauto. eapply lang_step_bind; eauto. }
+    { eapply IHSTEPS; eauto. }
+  }
+Qed.
+
+Lemma seq_thread_failure_bind R0 R1
+      (itr0 itr1: itree MemE.t R0) (k: R0 -> itree MemE.t R1)
+      mem0 p0 o0
+      (STEPS: SeqThread.failure
+                (@SeqState.na_step _)
+                (SeqThread.mk (@SeqState.mk (lang R0) itr0 mem0) p0 o0))
+  :
+    SeqThread.failure
+      (@SeqState.na_step _)
+      (@SeqThread.mk (lang R1) (@SeqState.mk (lang R1) (itr0 >>= k) mem0) p0 o0).
+Proof.
+  unfold SeqThread.failure in *. des. inv FAILURE. destruct st1.
+  esplits. econs. eapply na_step_bind; eauto.
 Qed.
 
 Lemma lang_step_deseq
@@ -202,139 +240,63 @@ Proof.
     right. right. splits; auto. f_equal. f_equal. extensionality v. ss. }
 Qed.
 
-Lemma thread_step_deseq
-      R0 R1 ktr (itr1: itree MemE.t R0) (itr2: itree MemE.t R1)
-      pf e
-      lc1 sc1 mem1
-      lc2 sc2 mem2
-      (STEP: Thread.step pf e
-                         (Thread.mk (lang _) (itr1 >>= ktr) lc1 sc1 mem1)
-                         (Thread.mk (lang _) itr2 lc2 sc2 mem2)):
-  (exists r,
-      itr1 = Ret r /\
-      Thread.step pf e
-                  (Thread.mk (lang _) (ktr r) lc1 sc1 mem1)
-                  (Thread.mk (lang _) (itr2) lc2 sc2 mem2)) \/
-  (exists itr2',
-      itr2 = itr2' >>= ktr /\
-      Thread.step pf e
-                  (Thread.mk (lang _) itr1 lc1 sc1 mem1)
-                  (Thread.mk (lang _) itr2' lc2 sc2 mem2)) \/
-  (itr1 = Vis MemE.abort (Empty_set_rect _) /\
-   e = ThreadEvent.failure)
-.
-Proof.
-  inv STEP.
-  - inv STEP0. right. left. esplits; eauto.
-    econs 1. econs; eauto.
-  - inv STEP0; ss.
-    apply lang_step_deseq in STATE. des; clarify.
-    { left. esplits; eauto. econs 2. econs; eauto. }
-    { right. left. esplits; eauto. econs 2. econs; eauto. }
-    { destruct e; ss; auto. }
-Qed.
 
-Lemma sim_rtc
-      A B
-      (sim:A -> B -> Prop)
-      (rA:A -> A -> Prop)
-      (rB:B -> B -> Prop)
-      (SIM:
-         forall a1 a2 b1 (RA: rA a1 a2) (SIM1: sim a1 b1),
-         exists b2, rB b1 b2 /\ sim a2 b2)
-      a1 a2 b1
-      (RA: rtc rA a1 a2) (SIM1: sim a1 b1):
-  exists b2, rtc rB b1 b2 /\ sim a2 b2.
-Proof.
-  revert b1 SIM1. induction RA; i.
-  - esplits; eauto.
-  - exploit SIM; eauto. i. des.
-    exploit IHRA; eauto. i. des.
-    esplits; [|eauto].
-    econs; eauto.
-Qed.
-
-Inductive sim_bind R0 R1 (k: R0 -> itree MemE.t R1):
-  forall (lhs: Thread.t (lang R0)) (rhs:Thread.t (lang R1)), Prop :=
-| sim_bind_intro
-    itr lc sc mem:
-    sim_bind k
-             (Thread.mk (lang R0) itr lc sc mem)
-             (Thread.mk (lang R1) (itr >>= k) lc sc mem)
-.
-
-Lemma rtc_internal_step_bind R0 R1
-      (itr0 itr1: itree MemE.t R0) (k: R0 -> itree MemE.t R1)
-      lc1 sc1 mem1
-      lc2 sc2 mem2
-      (STEP: rtc (@Thread.tau_step (lang R0))
-                 (Thread.mk (lang R0) itr0 lc1 sc1 mem1)
-                 (Thread.mk (lang R0) itr1 lc2 sc2 mem2)):
-  rtc (@Thread.tau_step (lang R1))
-      (Thread.mk (lang R1) (itr0 >>= k) lc1 sc1 mem1)
-      (Thread.mk (lang R1) (itr1 >>= k) lc2 sc2 mem2).
-Proof.
-  exploit (sim_rtc (sim_bind k)); eauto.
-  - i. inv SIM1. destruct a2. destruct local. inv RA. inv TSTEP.
-    generalize (step_bind k STEP0). i.
-    esplits; [|econs; eauto].
-    eapply tau_intro; eauto. eapply Thread.step_nopf_intro. eauto.
-  - econs; ss.
-  - i. des. inv x1. auto.
-Qed.
-
-
-Global Hint Resolve cpn11_wcompat: paco.
+Global Hint Resolve cpn7_wcompat: paco.
 
 Inductive ctx (sim_seq:SIM_SEQ): SIM_SEQ :=
 | ctx_ret
     R_src R_tgt
     (sim_ret:SIM_VAL R_src R_tgt)
-    sc0_src mem0_src
-    sc0_tgt mem0_tgt
-    lc_src lc_tgt (r_src: R_src) (r_tgt: R_tgt)
+    mem_src mem_tgt p
+    (r_src: R_src) (r_tgt: R_tgt)
     (RET: sim_ret r_src r_tgt)
-    (LOCAL: sim_local SimPromises.bot lc_src lc_tgt):
+    (VAL: ValueMap.le mem_tgt.(SeqMemory.value_map) mem_src.(SeqMemory.value_map))
+    (FLAG: Flags.le mem_tgt.(SeqMemory.flags) mem_src.(SeqMemory.flags)):
     @ctx sim_seq
          (lang R_src) (lang R_tgt)
          (sim_terminal sim_ret)
-         (Ret r_src) lc_src sc0_src mem0_src
-         (Ret r_tgt) lc_tgt sc0_tgt mem0_tgt
+         p Flags.bot
+         (@SeqState.mk (lang R_src) (Ret r_src) mem_src)
+         (@SeqState.mk (lang R_tgt) (Ret r_tgt) mem_tgt)
 | ctx_bind
     R_src0 R_tgt0 R_src1 R_tgt1
     (sim_ret1:SIM_VAL R_src0 R_tgt0) (sim_ret2:SIM_VAL R_src1 R_tgt1)
-    itr0 k0 lc_src sc0_src mem0_src
-    itr1 k1 lc_tgt sc0_tgt mem0_tgt
+    p f
+    itr_src ktr_src mem_src
+    itr_tgt ktr_tgt mem_tgt
     (SIM1: sim_seq (lang R_src0) (lang R_tgt0) (sim_terminal sim_ret1)
-                      itr0 lc_src sc0_src mem0_src
-                      itr1 lc_tgt sc0_tgt mem0_tgt)
-    (SIM2: _sim_ktree sim_seq sim_ret1 k0 k1 sim_ret2):
+                   p f
+                   (@SeqState.mk (lang R_src0) itr_src mem_src)
+                   (@SeqState.mk (lang R_tgt0) itr_tgt mem_tgt))
+    (SIM2: _sim_ktree sim_seq sim_ret1 ktr_src ktr_tgt sim_ret2):
     @ctx sim_seq
          (lang R_src1) (lang R_tgt1)
          (sim_terminal sim_ret2)
-         (itr0 >>= k0) lc_src sc0_src mem0_src
-         (itr1 >>= k1) lc_tgt sc0_tgt mem0_tgt
+         p f
+         (@SeqState.mk (lang R_src1) (itr_src >>= ktr_src) mem_src)
+         (@SeqState.mk (lang R_tgt1) (itr_tgt >>= ktr_tgt) mem_tgt)
 | ctx_tau_iter
     I_src I_tgt R_src R_tgt
     (sim_ret0: SIM_VAL I_src I_tgt) (sim_ret1: SIM_VAL R_src R_tgt)
-    sc0_src mem0_src
-    sc0_tgt mem0_tgt
-    lc_src lc_tgt
+    p
+    mem_src mem_tgt
     (body_src: I_src -> itree MemE.t (I_src + R_src))
     (body_tgt: I_tgt -> itree MemE.t (I_tgt + R_tgt))
     (SIM: _sim_ktree sim_seq sim_ret0 body_src body_tgt (sum_rel sim_ret0 sim_ret1))
     i_src i_tgt
     (VAL: sim_ret0 i_src i_tgt)
-    (LOCAL: sim_local SimPromises.bot lc_src lc_tgt)
+    (VALS: ValueMap.le mem_tgt.(SeqMemory.value_map) mem_src.(SeqMemory.value_map))
+    (FLAG: Flags.le mem_tgt.(SeqMemory.flags) mem_src.(SeqMemory.flags))
   :
     @ctx sim_seq
-              (lang R_src) (lang R_tgt)
-              (sim_terminal sim_ret1)
-              (tau;;(ITree.iter body_src i_src)) lc_src sc0_src mem0_src
-              (tau;;(ITree.iter body_tgt i_tgt)) lc_tgt sc0_tgt mem0_tgt
+         (lang R_src) (lang R_tgt)
+         (sim_terminal sim_ret1)
+         p Flags.bot
+         (@SeqState.mk (lang _) (tau;;(ITree.iter body_src i_src)) mem_src)
+         (@SeqState.mk (lang _) (tau;;(ITree.iter body_tgt i_tgt)) mem_tgt)
 .
 
-Lemma ctx_mon: monotone11 ctx.
+Lemma ctx_mon: monotone7 ctx.
 Proof.
   ii. destruct IN.
   - econs 1; eauto.
@@ -356,206 +318,269 @@ Proof.
   eapply bisimulation_is_eq. eapply unfold_iter.
 Qed.
 
-Lemma ctx_compat:
-  ctx <12= gupaco11 _sim_seq (cpn11 _sim_seq).
+
+Inductive ctx_src_steps (sim_seq:SIM_SEQ): SIM_SEQ :=
+| ctx_src_steps_intro
+    lang_src lang_tgt sim_terminal
+    th_src0 th_src1 th_tgt p f
+    (STEPS: rtc (SeqState.na_step p MachineEvent.silent) th_src0 th_src1)
+    (SIM: @sim_seq lang_src lang_tgt sim_terminal p f th_src1 th_tgt)
+  :
+    @ctx_src_steps
+      sim_seq
+      lang_src lang_tgt
+      sim_terminal
+      p f
+      th_src0
+      th_tgt
+.
+
+Lemma ctx_src_mon: monotone7 ctx_src_steps.
 Proof.
-  assert (MON: monotone11 _sim_seq).
+  ii. destruct IN. econs; eauto.
+Qed.
+Hint Resolve ctx_src_mon.
+
+Lemma na_steps_thread_steps lang th_src0 th_src1 th_src2 tr p0 o0
+      (STEPS0: rtc (SeqState.na_step p0 MachineEvent.silent) th_src0 th_src1)
+      (STEPS1: SeqThread.steps (@SeqState.na_step lang) tr
+                               (@SeqThread.mk lang th_src1 p0 o0) th_src2)
+  :
+    SeqThread.steps (@SeqState.na_step lang) tr (@SeqThread.mk lang th_src0 p0 o0) th_src2.
+Proof.
+  induction STEPS0; auto. econs 2.
+  { econs; eauto. }
+  { eauto. }
+Qed.
+
+Lemma ctx_src_steps_compat:
+  ctx_src_steps <8= gupaco7 _sim_seq (cpn7 _sim_seq).
+Proof.
+  assert (MON: monotone7 _sim_seq).
   (* paco tactics do not work well without this *)
-  { eapply _sim_seq_mon; eauto. }
-  eapply wrespect11_uclo; auto.
+  { eapply sim_seq_mon; eauto. }
+  eapply grespect7_uclo; auto.
+  econs; auto. i. destruct PR. eapply rclo7_base.
+  eapply GF in SIM. inv SIM.
+  { econs 1.
+    { ii. exploit TERMINAL; eauto. i. des. esplits.
+      { etrans; eauto. }
+      { eauto. }
+      { eauto. }
+      { eauto. }
+      { eauto. }
+    }
+    { ii. exploit NASTEP; eauto. i. des. esplits.
+      { etrans; eauto. }
+      { eauto. }
+      { eapply rclo7_base. auto. }
+    }
+    { ii. exploit ATSTEP; eauto. i. des. esplits.
+      { etrans; eauto. }
+      { eauto. }
+      { eauto. }
+      { i. exploit SIM; eauto. i. des. esplits; eauto.
+        eapply rclo7_base; auto. }
+    }
+    { ii. exploit PARTIAL; eauto. i. des.
+      { esplits; eauto. eapply na_steps_thread_steps; eauto. }
+      { esplits; eauto. eapply na_steps_thread_steps; eauto. }
+    }
+  }
+  { econs 2. ii. exploit FAILURE; eauto. i. des.
+    esplits; eauto. eapply na_steps_thread_steps; eauto.
+  }
+Qed.
+
+Lemma ctx_compat:
+  ctx <8= gupaco7 _sim_seq (cpn7 _sim_seq).
+Proof.
+  assert (MON: monotone7 _sim_seq).
+  (* paco tactics do not work well without this *)
+  { eapply sim_seq_mon; eauto. }
+  eapply grespect7_uclo; auto.
   econs; auto. i. destruct PR.
   - (* ret *)
-    ii.
-    inversion LOCAL. apply SimPromises.sem_bot_inv in PROMISES; auto.
-    destruct lc_src, lc_tgt. ss. subst.
-    splits; s; ii.
-    { right. inv TERMINAL_TGT. ss. esplits; eauto; ss.
-      - econs; eauto.
-      - econs; eauto.
+    eapply rclo7_base. econs.
+    { ii. ss. inv TERMINAL_TGT. clarify. esplits; ss.
+      { refl. }
+      { ss. econs; eauto. }
+      { ss. econs; eauto. }
+      { ss. }
+      { ss. }
     }
-    { right. subst. esplits; eauto. }
-    inv STEP_TGT; try by inv STEP; inv STATE.
-    inv STEP; ss.
-    exploit sim_local_promise; eauto. i. des.
-    right. esplits.
-    + ss.
-    + eauto.
-    + econs 2. econs 1. econs; eauto.
-    + eauto.
-    + eauto.
-    + eauto.
-    + eapply rclo11_clo_base. eapply ctx_ret; auto.
+    { ii. inv STEP_TGT. inv LANG. }
+    { ii. inv STEP_TGT. }
+    { ii. esplits; ss.
+      { econs 1. }
+      { econs. }
+      { ss. left. eapply Flags.join_mon_r. auto. }
+    }
   - (* bind *)
-    ii. ss. eapply GF in SIM1.
-    exploit SIM1; try apply SC; eauto. i. des.
-    splits; s; ii.
-    { inv TERMINAL_TGT. ides itr1.
-      2: { eapply f_equal with (f:=observe) in H. ss. }
-      2: { eapply f_equal with (f:=observe) in H. ss. }
-      rewrite bind_ret_l in H.
-      exploit TERMINAL; try by econs. i. des.
-      - left.
-        unfold Thread.steps_failure in *. des.
-        destruct e2, e3.
-        eapply rtc_internal_step_bind in STEPS.
-        eapply step_bind in STEP_FAILURE.
-        esplits; eauto.
-      - inversion LOCAL. exploit SimPromises.sem_bot_inv; eauto. i.
-        destruct lc2_src. ss. subst.
-        inv TERMINAL_SRC.
-        exploit Thread.rtc_tau_step_future; eauto. s. i. des.
-        inv TERMINAL0. ss.
-        assert (x0 = r1).
-        { eapply f_equal with (f:=observe) in SRC. ss. clarify. }
-        assert (r0 = r2).
-        { eapply f_equal with (f:=observe) in TGT. ss. clarify. }
-        subst.
-        exploit SIM2; eauto. i. eapply GF in x0.
-        exploit x0; try apply SC0; eauto using Memory.future_future_weak.
-        i. ss. des. exploit TERMINAL0; try by econs.
-        { econs. eauto. }
-        i. des.
-        + left.
-          unfold Thread.steps_failure in *. des.
-          destruct e2.
-          esplits; [|eauto|eauto].
-          etrans; try exact STEPS0.
-          eapply rtc_internal_step_bind in STEPS.
-          rewrite bind_ret_l in STEPS. eauto.
-        + right.
-          destruct lc2_src.
-          esplits; cycle 1; eauto.
-          * rewrite bind_ret_l. eauto.
-          * etrans; [|eauto].
-            eapply rtc_internal_step_bind in STEPS.
-            rewrite bind_ret_l in STEPS. eauto.
+    destruct (classic (exists r, itr_tgt = Ret r)).
+    { des; clarify. eapply GF in SIM1. inv SIM1; cycle 1.
+      { eapply rclo7_base. econs 2. ii.
+        exploit FAILURE; eauto. i. des.
+        destruct th. destruct state0. esplits.
+        { eapply seq_thread_steps_bind in STEPS; eauto. }
+        { eauto. }
+        { eapply seq_thread_failure_bind; eauto. }
+      }
+      exploit TERMINAL; eauto.
+      { econs; eauto; ss. }
+      i. des. eapply rclo7_clo.
+      eapply cpn7_gupaco; eauto.
+      destruct st_src1. ss. eapply rtc_na_step_bind in STEPS.
+      guclo ctx_src_steps_compat. econs.
+      { eauto. }
+      inv TERMINAL0. clarify. rewrite bind_ret_l. rewrite bind_ret_l.
+      guclo deferred_le_sf_ctx_spec. econs.
+      { instantiate (1:=Flags.bot). ss. etrans; eauto.
+        eapply Flags.join_ge_l.
+      }
+      guclo mem_le_ctx_spec. econs; ss; eauto.
+      { instantiate (1:=SeqState.mk _ _ _). ss. red. splits; eauto.
+        etrans; eauto. eapply Flags.join_ge_r.
+      }
+      { ss. }
+      exploit SIM2; eauto. i.
+      gbase. eapply rclo7_base. eapply GF in x.
+      eapply sim_seq_mon; eauto.
+      i. eapply rclo7_base. auto.
     }
-    { exploit PROMISES; eauto. i. des.
-      - left.
-        unfold Thread.steps_failure in *. des.
-        destruct e2, e3.
-        eapply rtc_internal_step_bind in STEPS.
-        eapply step_bind in STEP_FAILURE.
-        esplits; eauto.
-      - right.
-        destruct lc_tgt, lc2_src. ss. subst.
-        esplits; [|eauto].
-        + eapply rtc_internal_step_bind. apply STEPS.
-        + ss.
-    }
-    hexploit thread_step_deseq; eauto. i. des; clarify.
-    + exploit TERMINAL; try by econs. i. des.
-      * left.
-        unfold Thread.steps_failure in *. des.
-        destruct e2, e3. ss.
-        eapply rtc_internal_step_bind in STEPS.
-        eapply step_bind in STEP_FAILURE.
-        esplits; eauto.
-      * inversion LOCAL. exploit SimPromises.sem_bot_inv; eauto. i. subst.
-        destruct lc2_src. inv TERMINAL_SRC. ss. subst.
-        exploit Thread.rtc_tau_step_future; eauto. s. i. des.
-        inv TERMINAL0. ss. subst.
-        assert (x = r1).
-        { eapply f_equal with (f:=observe) in SRC. ss. clarify. }
-        assert (r0 = r2).
-        { eapply f_equal with (f:=observe) in TGT. ss. clarify. }
-        subst.
-        exploit SIM2; eauto. i. eapply GF in x.
-        exploit x; try apply SC0; eauto using Memory.future_future_weak.
-        i. ss. des.
-        exploit STEP0; eauto. i. des.
-        { left.
-          unfold Thread.steps_failure in *. des.
-          destruct e2, e3.
-          eapply rtc_internal_step_bind in STEPS.
-          esplits; try exact STEP_FAILURE; [|eauto].
-          etrans; eauto. rewrite bind_ret_l. eauto. }
-        { right.
-          esplits; cycle 2; eauto.
-          - eapply rclo11_base. auto.
-          - eapply rtc_internal_step_bind in STEPS.
-            etrans; [apply STEPS|eauto].
-            rewrite bind_ret_l. eauto. }
-    + destruct lc3_tgt.
-      exploit STEP; eauto. i. des.
-      * left.
-        unfold Thread.steps_failure in *. des.
-        destruct e2, e3.
-        eapply rtc_internal_step_bind in STEPS.
-        eapply step_bind in STEP_FAILURE.
-        esplits; eauto.
-      * right.
-        destruct lc2_src. destruct lc3_src.
-        esplits; [|M|M| | | |]; Mskip eauto.
-        { eapply rtc_internal_step_bind. eauto. }
-        { eapply opt_step_bind. eauto. }
-        { eapply rclo11_clo_base. eapply ctx_bind; eauto.
-          eapply _sim_ktree_mon; cycle 1; eauto.
+    destruct (classic (sim_seq_failure_case p (@SeqState.mk (lang R_src1) (itr_src >>= ktr_src) mem_src))).
+    { eapply rclo7_base. econs 2; eauto. }
+    { eapply rclo7_base. eapply GF in SIM1. inv SIM1.
+      { econs.
+        { ii. inv TERMINAL_TGT; ss. exfalso.
+          eapply f_equal with (f:=observe) in H1.
+          ides itr_tgt; eauto.
         }
-    + left. exploit STEP.
-      { right. instantiate (5:=ThreadEvent.failure). econs; eauto.
-        ss. econs; eauto. }
-      i. des; ss.
-      unfold Thread.steps_failure in *. des. destruct e2, e3. esplits; [..|eauto].
-      { eapply rtc_internal_step_bind; eauto. }
-      { eapply step_bind; eauto. }
-  - (* tau iter *)
-    ii.
-    inversion LOCAL. exploit SimPromises.sem_bot_inv; eauto. i.
-    destruct lc_src, lc_tgt. ss. subst.
-    splits; s; ii.
-    { inv TERMINAL_TGT. eapply f_equal with (f:=observe) in H. ss. }
-    { right. subst. esplits; eauto. }
-    right. inv STEP_TGT; ss.
-    + (* promise *)
-      inv STEP; ss.
-      exploit sim_local_promise; eauto. i. des.
-      esplits; try apply SC; eauto; ss.
-      { econs 2. econs 1. econs; eauto. }
-      { eauto. }
-      { eapply rclo11_clo_base. eapply ctx_tau_iter; eauto.
-        eapply _sim_ktree_mon; cycle 1; eauto.
+        { ii. inv STEP_TGT. apply lang_step_deseq in LANG. des; clarify.
+          { exfalso. eauto. }
+          { exploit NASTEP; eauto.
+            { econs; eauto. }
+            i. des. destruct st_src1, st_src2. esplits.
+            { eapply rtc_na_step_bind; eauto. }
+            { eapply na_opt_step_bind; eauto. }
+            { eapply rclo7_clo. right.
+              gbase. eapply rclo7_clo_base.
+              { left. econs.
+                { eauto. }
+                { eapply _sim_ktree_mon; eauto. }
+              }
+            }
+          }
+          { exploit NASTEP; eauto.
+            { econs; eauto. econs; eauto. }
+            i. des. inv LOCAL. inv STEP.
+            exfalso. eapply H0. ii.
+            destruct st_src1, st_src2. exploit na_steps_thread_steps.
+            { eauto. }
+            { econs 1. }
+            i. esplits.
+            { eapply seq_thread_steps_bind; eauto. }
+            { econs. }
+            { econs. econs. eapply na_step_bind; eauto. }
+          }
+        }
+        { ii. apply lang_step_deseq in STEP_TGT. des; clarify; ss.
+          { exfalso. eauto. }
+          exploit ATSTEP; eauto.
+          i. des. destruct st_src1. esplits.
+          { eapply rtc_na_step_bind; eauto. }
+          { eapply lang_step_bind; eauto. }
+          { eauto. }
+          { i. exploit SIM; eauto. i. des. esplits; eauto.
+            eapply rclo7_clo. right.
+            gbase. eapply rclo7_clo_base.
+            { left. econs.
+              { eauto. }
+              { eapply _sim_ktree_mon; eauto. }
+            }
+          }
+        }
+        { ii. exploit PARTIAL; eauto. i. des.
+          { destruct th. destruct state0. ss. esplits; eauto.
+            { eapply seq_thread_steps_bind; eauto. }
+            { ss. left. auto. }
+          }
+          { destruct th. destruct state0. ss. esplits; eauto.
+            { eapply seq_thread_steps_bind; eauto. }
+            { ss. right. eapply seq_thread_failure_bind; eauto. }
+          }
+        }
       }
-    + (* tau *)
-      inv STEP. ss. inv LOCAL0; dependent destruction STATE.
-      inv LOCAL; ss.
-      esplits; try apply SC; eauto; ss.
-      { econs 2. econs 2. econs; [|econs 1]; eauto. econs; eauto. }
-      { eauto. }
-      { rewrite unfold_iter_eq. rewrite unfold_iter_eq.
-        eapply rclo11_clo. eapply ctx_bind; eauto.
-        { eapply rclo11_base. eapply LE. eapply SIM; ss. }
-        ii. eapply rclo11_clo. inv RET.
-        { eapply ctx_tau_iter; eauto.
-          eapply _sim_ktree_mon; cycle 1; eauto.
-          i. eapply rclo11_base. eauto. }
-        { eapply ctx_ret; eauto. }
+      { econs 2. ii. exploit FAILURE; eauto. i. des.
+        destruct th. ss. destruct state0. esplits.
+        { eapply seq_thread_steps_bind in STEPS; eauto. }
+        { eauto. }
+        { eapply seq_thread_failure_bind; eauto. }
       }
-  Unshelve. all: try exact ITree.spin.
+    }
+  - (* iter *)
+    eapply rclo7_base. econs.
+    { ii. ss. inv TERMINAL_TGT. clarify. }
+    { ii. inv STEP_TGT. inv LANG. inv LOCAL. esplits.
+      { refl. }
+      { econs 1. econs.
+        { econs; eauto. }
+        { econs. }
+      }
+      { eapply rclo7_clo. left.
+        rewrite unfold_iter_eq. rewrite unfold_iter_eq. econs.
+        { eapply rclo7_clo_base. right.
+          guclo deferred_le_sf_ctx_spec. econs.
+          { ss. }
+          guclo mem_le_ctx_spec. econs.
+          3:{ gbase. eapply LE. eapply SIM; eauto. }
+          { ss. }
+          { ss. }
+        }
+        { ii. inv RET.
+          { eapply rclo7_clo_base. left. econs 3; eauto.
+            { eapply _sim_ktree_mon; eauto. }
+            { refl. }
+            { refl. }
+          }
+          { eapply rclo7_clo_base. left. econs 1; eauto.
+            { refl. }
+            { refl. }
+          }
+        }
+      }
+    }
+    { ii. inv STEP_TGT. ss. }
+    { ii. esplits.
+      { econs 1. }
+      { econs. }
+      { left. ss. }
+    }
 Qed.
 
 Inductive iter_ctx (sim_seq:SIM_SEQ): SIM_SEQ :=
 | ctx_iter
     I_src I_tgt R_src R_tgt
     (sim_ret0: SIM_VAL I_src I_tgt) (sim_ret1: SIM_VAL R_src R_tgt)
-    sc0_src mem0_src
-    sc0_tgt mem0_tgt
-    lc_src lc_tgt
+    p
+    mem_src mem_tgt
     (body_src: I_src -> itree MemE.t (I_src + R_src))
     (body_tgt: I_tgt -> itree MemE.t (I_tgt + R_tgt))
     (SIM: _sim_ktree sim_seq sim_ret0 body_src body_tgt (sum_rel sim_ret0 sim_ret1))
     i_src i_tgt
     (VAL: sim_ret0 i_src i_tgt)
-    (LOCAL: sim_local SimPromises.bot lc_src lc_tgt)
+    (VALS: ValueMap.le mem_tgt.(SeqMemory.value_map) mem_src.(SeqMemory.value_map))
+    (FLAG: Flags.le mem_tgt.(SeqMemory.flags) mem_src.(SeqMemory.flags))
   :
     @iter_ctx sim_seq
               (lang R_src) (lang R_tgt)
               (sim_terminal sim_ret1)
-              (ITree.iter body_src i_src) lc_src sc0_src mem0_src
-              (ITree.iter body_tgt i_tgt) lc_tgt sc0_tgt mem0_tgt
+              p Flags.bot
+              (@SeqState.mk (lang _) ((ITree.iter body_src i_src)) mem_src)
+              (@SeqState.mk (lang _) ((ITree.iter body_tgt i_tgt)) mem_tgt)
 .
 
-Lemma iter_ctx_mon: monotone11 iter_ctx.
+Lemma iter_ctx_mon: monotone7 iter_ctx.
 Proof.
   ii. destruct IN.
   econs; eauto. ii. eapply LE. eapply SIM; eauto.
@@ -563,113 +588,182 @@ Qed.
 Hint Resolve iter_ctx_mon.
 
 Lemma iter_ctx_compat:
-  iter_ctx <12= gupaco11 _sim_seq (cpn11 _sim_seq).
+  iter_ctx <8= gupaco7 _sim_seq (cpn7 _sim_seq).
 Proof.
-  assert (MON: monotone11 _sim_seq).
+  assert (MON: monotone7 _sim_seq).
   (* paco tactics do not work well without this *)
-  { eapply _sim_seq_mon; eauto. }
-  eapply grespect11_uclo; auto.
+  { eapply sim_seq_mon; eauto. }
+  eapply grespect7_uclo; auto.
   econs; auto. i. destruct PR.
-  eapply rclo11_clo_base. eapply cpn11_gupaco; [eauto with paco|].
+  eapply rclo7_clo_base. eapply cpn7_gupaco; [eauto with paco|].
   rewrite unfold_iter_eq. rewrite unfold_iter_eq.
   guclo ctx_compat. eapply ctx_bind.
-  { gbase. eapply _sim_seq_mon.
+  { guclo mem_le_ctx_spec. econs.
+    { instantiate (1:=SeqState.mk _ _ mem_tgt).
+      red. splits; ss; eauto.
+    }
+    { ss. }
+    gbase. eapply sim_seq_mon.
     { hexploit (@SIM i_src i_tgt); eauto. }
-    { i. eapply rclo11_base. eauto. }
+    { i. eapply rclo7_base. eauto. }
   }
   { ii. inv RET.
     { guclo ctx_compat. eapply ctx_tau_iter; eauto.
-      eapply _sim_ktree_mon; cycle 1; eauto.
-      i. gbase. eapply _sim_seq_mon; eauto.
-      i. eapply rclo11_base. eauto.
+      { eapply _sim_ktree_mon; cycle 1; eauto.
+        i. gbase. eapply sim_seq_mon; eauto.
+        i. eapply rclo7_base. eauto.
+      }
+      { refl. }
+      { refl. }
     }
-    { guclo ctx_compat. eapply ctx_ret; eauto. }
+    { guclo ctx_compat. eapply ctx_ret; eauto.
+      { refl. }
+      { refl. }
+    }
   }
 Qed.
 
-Definition sim_itree := @_sim_itree sim_seq.
-Definition sim_ktree := @_sim_ktree sim_seq.
+Definition sim_seq_itree := @_sim_itree sim_seq.
+Definition sim_seq_ktree := @_sim_ktree sim_seq.
 
-Lemma sim_itree_mon R_src R_tgt
+Lemma sim_seq_mon lang_src lang_tgt sim_terminal0 sim_terminal1
+      p f th_src th_tgt
+      (SIM01: sim_terminal0 <2= sim_terminal1)
+      (SIM: @sim_seq lang_src lang_tgt sim_terminal0 p f th_src th_tgt):
+  @sim_seq lang_src lang_tgt sim_terminal1 p f th_src th_tgt.
+Proof.
+  revert p f th_src th_tgt SIM. pcofix CIH. i.
+  punfold SIM. pfold. inv SIM.
+  { econs 1.
+    { ii. exploit TERMINAL; eauto.
+      i. des. esplits; eauto.
+    }
+    { ii. exploit NASTEP; eauto. i. des. esplits; eauto.
+      pclearbot. right. eapply CIH; eauto.
+    }
+    { ii. exploit ATSTEP; eauto. i. des. esplits; eauto.
+      i. exploit SIM; eauto. i. des. esplits; eauto.
+      pclearbot. right. eapply CIH; eauto.
+    }
+    { ii. exploit PARTIAL; eauto. }
+  }
+  { econs 2. auto. }
+Qed.
+
+Lemma sim_seq_itree_mon R_src R_tgt
       sim_ret0 sim_ret1
       itr_src itr_tgt
       (SIM01: sim_ret0 <2= sim_ret1)
-      (SIM: @sim_itree R_src R_tgt sim_ret0 itr_src itr_tgt):
-  sim_itree sim_ret1 itr_src itr_tgt.
+      (SIM: @sim_seq_itree R_src R_tgt sim_ret0 itr_src itr_tgt):
+  sim_seq_itree sim_ret1 itr_src itr_tgt.
 Proof.
-  ii. eapply sim_seq_mon; [|eauto].
+  ii. eapply sim_seq_mon.
+  2:{ eauto. }
   i. inv PR. econs; eauto.
 Qed.
 
-Lemma sim_itree_ret R_src R_tgt (sim_ret: SIM_VAL R_src R_tgt)
-      r_src r_tgt
-      (SIM: sim_ret r_src r_tgt):
-  @sim_itree R_src R_tgt sim_ret (Ret r_src) (Ret r_tgt).
+Lemma sim_itree_refl R (itr: itree MemE.t R)
+  :
+    sim_seq_itree eq itr itr.
 Proof.
-  ii. ginit. guclo ctx_compat. econs 1; eauto.
+  ii. generalize (@SeqState.mk (lang R) itr mem). revert p. clear itr mem.
+  pcofix CIH. pfold. econs.
+  { ii. inv TERMINAL_TGT. esplits; eauto.
+    { econs; eauto. }
+    { econs; eauto. }
+    { refl. }
+    { refl. }
+  }
+  { ii. esplits; eauto.
+    { econs; eauto. }
+  }
+  { ii. esplits; eauto.
+    { refl. }
+    { i. esplits; eauto. eapply SeqEvent.input_match_bot. }
+  }
+  { ii. esplits; eauto.
+    { econs. }
+    { econs. }
+    { left. ss. refl. }
+  }
 Qed.
 
-Lemma sim_itree_bind
+Lemma sim_seq_itree_ret R_src R_tgt (sim_ret: SIM_VAL R_src R_tgt)
+      r_src r_tgt
+      (SIM: sim_ret r_src r_tgt):
+  @sim_seq_itree R_src R_tgt sim_ret (Ret r_src) (Ret r_tgt).
+Proof.
+  ii. ginit. guclo ctx_compat. econs 1; eauto.
+  { refl. }
+  { refl. }
+Qed.
+
+Lemma sim_seq_itree_bind
       R_src0 R_tgt0 R_src1 R_tgt1
       (sim_ret0: SIM_VAL R_src0 R_tgt0)
       (sim_ret1: SIM_VAL R_src1 R_tgt1)
       itr_src itr_tgt k_src k_tgt
-      (SIM1: sim_itree sim_ret0 itr_src itr_tgt)
-      (SIM2: sim_ktree sim_ret0 k_src k_tgt sim_ret1):
-  sim_itree sim_ret1 (itr_src >>= k_src) (itr_tgt >>= k_tgt).
+      (SIM1: sim_seq_itree sim_ret0 itr_src itr_tgt)
+      (SIM2: sim_seq_ktree sim_ret0 k_src k_tgt sim_ret1):
+  sim_seq_itree sim_ret1 (itr_src >>= k_src) (itr_tgt >>= k_tgt).
 Proof.
   ii. ginit. guclo ctx_compat. econs 2.
   - gfinal. right. apply SIM1; auto.
   - ii. gfinal. right. apply SIM2; auto.
 Qed.
 
-Lemma sim_itree_iter
+Lemma sim_seq_itree_iter
       I_src I_tgt R_src R_tgt
       (sim_ret0: SIM_VAL I_src I_tgt) (sim_ret1: SIM_VAL R_src R_tgt)
       (body_src: I_src -> itree MemE.t (I_src + R_src))
       (body_tgt: I_tgt -> itree MemE.t (I_tgt + R_tgt))
-      (SIM: sim_ktree sim_ret0 body_src body_tgt (sum_rel sim_ret0 sim_ret1))
+      (SIM: sim_seq_ktree sim_ret0 body_src body_tgt (sum_rel sim_ret0 sim_ret1))
       i_src i_tgt
       (VAL: sim_ret0 i_src i_tgt):
-  sim_itree sim_ret1 (ITree.iter body_src i_src) (ITree.iter body_tgt i_tgt).
+  sim_seq_itree sim_ret1 (ITree.iter body_src i_src) (ITree.iter body_tgt i_tgt).
 Proof.
   ii. ginit. guclo iter_ctx_compat. econs; eauto.
-  eapply _sim_ktree_mon; cycle 1; eauto.
-  ii. gfinal. right. eauto.
+  { eapply _sim_ktree_mon; cycle 1; eauto.
+    ii. gfinal. right. eauto. }
+  { refl. }
+  { refl. }
 Qed.
 
-
-Lemma sim_ktree_ret R_src R_tgt sim_ret:
-  @sim_ktree R_src R_tgt R_src R_tgt sim_ret (fun r => Ret r) (fun r => Ret r) sim_ret.
+Lemma sim_seq_ktree_ret R_src R_tgt sim_ret:
+  @sim_seq_ktree R_src R_tgt R_src R_tgt sim_ret (fun r => Ret r) (fun r => Ret r) sim_ret.
 Proof.
   ii. ginit. guclo ctx_compat. econs 1; eauto.
+  { refl. }
+  { refl. }
 Qed.
 
-Lemma sim_ktree_bind
+Lemma sim_seq_ktree_bind
       R_src0 R_tgt0 R_src1 R_tgt1 R_src2 R_tgt2
       (sim_ret0: SIM_VAL R_src0 R_tgt0)
       (sim_ret1: SIM_VAL R_src1 R_tgt1)
       (sim_ret2: SIM_VAL R_src2 R_tgt2)
       k1_src k2_src
       k1_tgt k2_tgt
-      (SIM1: sim_ktree sim_ret0 k1_src k1_tgt sim_ret1)
-      (SIM2: sim_ktree sim_ret1 k2_src k2_tgt sim_ret2):
-  sim_ktree sim_ret0 (fun r => k1_src r >>= k2_src) (fun r => k1_tgt r >>= k2_tgt) sim_ret2.
+      (SIM1: sim_seq_ktree sim_ret0 k1_src k1_tgt sim_ret1)
+      (SIM2: sim_seq_ktree sim_ret1 k2_src k2_tgt sim_ret2):
+  sim_seq_ktree sim_ret0 (fun r => k1_src r >>= k2_src) (fun r => k1_tgt r >>= k2_tgt) sim_ret2.
 Proof.
   ii. ginit. guclo ctx_compat. econs 2.
   - gfinal. right. apply SIM1; auto.
   - ii. gfinal. right. apply SIM2; auto.
 Qed.
 
-Lemma sim_ktree_iter
+Lemma sim_seq_ktree_iter
       I_src I_tgt R_src R_tgt
       (sim_ret0: SIM_VAL I_src I_tgt) (sim_ret1: SIM_VAL R_src R_tgt)
       (body_src: I_src -> itree MemE.t (I_src + R_src))
       (body_tgt: I_tgt -> itree MemE.t (I_tgt + R_tgt))
-      (SIM: sim_ktree sim_ret0 body_src body_tgt (sum_rel sim_ret0 sim_ret1)):
-  sim_ktree sim_ret0 (ITree.iter body_src) (ITree.iter body_tgt) sim_ret1.
+      (SIM: sim_seq_ktree sim_ret0 body_src body_tgt (sum_rel sim_ret0 sim_ret1)):
+  sim_seq_ktree sim_ret0 (ITree.iter body_src) (ITree.iter body_tgt) sim_ret1.
 Proof.
   ii. ginit. guclo iter_ctx_compat. econs; eauto.
-  eapply _sim_ktree_mon; cycle 1; eauto.
-  ii. gfinal. right. eauto.
+  { eapply _sim_ktree_mon; cycle 1; eauto.
+    ii. gfinal. right. eauto. }
+  { refl. }
+  { refl. }
 Qed.
